FOL/Computing/EpsilonNFA.lean
@@ -4,7 +4,7 @@ import FOL.Computing.DFS
 set_option autoImplicit false
 
 
-structure SymbolStepMultiple
+structure SymbolArrow
   (α : Type)
   [DecidableEq α]
   (σ : Type)
@@ -12,136 +12,64 @@ structure SymbolStepMultiple
   Type :=
   (start_state : σ)
   (symbol : α)
-  (stop_state_list : List σ)
-  deriving Repr
-
-
-structure EpsilonStepMultiple
-  (σ : Type)
-  [DecidableEq σ] :
-  Type :=
-  (start_state : σ)
-  (stop_state_list : List σ)
-  deriving Repr
-
-
-structure EpsilonNFA
-  (α : Type)
-  [DecidableEq α]
-  (σ : Type)
-  [DecidableEq σ] :
-  Type :=
-  (symbol_step_list : List (SymbolStepMultiple α σ))
-  (epsilon_step_list : List (EpsilonStepMultiple σ))
-  (starting_state_list : List σ)
-  (accepting_state_list : List σ)
-  deriving Repr
-
-
-structure EpsilonStepSingle
-  (σ : Type)
-  [DecidableEq σ] :
-  Type :=
-  (start_state : σ)
   (stop_state : σ)
   deriving Repr
 
 
 /--
-  Translates an epsilon step that is from a single state to a list of states, to a list of epsilon steps that are each from a single state to a single state.
--/
-def epsilon_step_multiple_to_single_list
-  {σ : Type}
-  [DecidableEq σ]
-  (step : EpsilonStepMultiple σ) :
-  List (EpsilonStepSingle σ) :=
-  step.stop_state_list.map (fun (stop_state : σ) =>
-    ⟨
-      step.start_state,
-      stop_state
-    ⟩ )
-
-
-/--
-  Translates a list of epsilon steps that are each from a single state to a list of states, to a list of epsilon steps that are each from a single state to a single state.
--/
-def epsilon_step_multiple_list_to_single_list
-  {σ : Type}
-  [DecidableEq σ]
-  (step_list : List (EpsilonStepMultiple σ)) :
-  List (EpsilonStepSingle σ) :=
-  (step_list.map (fun (step : EpsilonStepMultiple σ) => epsilon_step_multiple_to_single_list step)).join
-
-
-/--
-  Translates a list of epsilon steps that are each from a single state to a single state, to an adjacency list representation of a graph.
--/
-def epsilon_step_single_list_to_graph
-  {σ : Type}
-  [DecidableEq σ]
-  (step_list : List (EpsilonStepSingle σ)) :
-  Graph σ :=
-    step_list.map (fun (step : (EpsilonStepSingle σ)) => (step.start_state, step.stop_state))
-
-
-/--
-  Translates a list of epsilon steps that are each from a single state to a list of states, to an adjacency list representation of a graph.
--/
-def epsilon_step_multiple_list_to_graph
-  {σ : Type}
-  [DecidableEq σ]
-  (step_list : List (EpsilonStepMultiple σ)) :
-  Graph σ :=
-  epsilon_step_single_list_to_graph (epsilon_step_multiple_list_to_single_list step_list)
-
-
-/--
-  Takes a list of epsilon steps that are each from a single state to a list of states and calculates the epsilon closure of a set of states with respect to the graph generated from the list of epsilon steps.
--/
-def epsilon_closure
-  {σ : Type}
-  [DecidableEq σ]
-  (epsilon_step_list : List (EpsilonStepMultiple σ))
-  (state_list : List σ) :
-  List σ :=
-    dfs_aux (epsilon_step_multiple_list_to_graph epsilon_step_list) state_list []
-
-
-/--
   The accumulated stop states of all of the steps in the list that have a start state and symbol matching the given state and symbol.
 -/
-def symbol_step_multiple_list_to_fun
+def symbol_arrow_list_to_fun
   {α : Type}
   [DecidableEq α]
   {σ : Type}
   [DecidableEq σ]
-  (step_list : List (SymbolStepMultiple α σ))
+  (symbol_arrow_list : List (SymbolArrow α σ))
   (state : σ)
   (symbol : α) :
   List σ :=
-  (step_list.filterMap (fun (step : SymbolStepMultiple α σ) =>
-    if step.start_state = state ∧ step.symbol = symbol
-    then Option.some step.stop_state_list
-    else Option.none)).join
+  (symbol_arrow_list.filterMap (fun (arrow : SymbolArrow α σ) =>
+    if arrow.start_state = state ∧ arrow.symbol = symbol
+    then Option.some arrow.stop_state
+    else Option.none)).dedup
 
 
-example : symbol_step_multiple_list_to_fun ([] : List (SymbolStepMultiple Char Nat)) 0 'a' == [] := by rfl
+example : symbol_arrow_list_to_fun ([] : List (SymbolArrow Char Nat)) 0 'a' = [] := by rfl
 
-example : symbol_step_multiple_list_to_fun [⟨0, 'a', [1]⟩] 0 'a' == [1] := by rfl
+example : symbol_arrow_list_to_fun [⟨0, 'a', 1⟩] 0 'a' = [1] := by rfl
 
-example : symbol_step_multiple_list_to_fun [⟨0, 'a', [1]⟩] 0 'b' == [] := by rfl
+example : symbol_arrow_list_to_fun [⟨0, 'a', 1⟩] 0 'b' = [] := by rfl
 
-example : symbol_step_multiple_list_to_fun [⟨0, 'a', [1]⟩, ⟨0, 'b', [1]⟩] 0 'a' == [1] := by rfl
+example : symbol_arrow_list_to_fun [⟨0, 'a', 1⟩, ⟨0, 'b', 1⟩] 0 'a' = [1] := by rfl
 
-example : symbol_step_multiple_list_to_fun [⟨0, 'a', [1]⟩, ⟨0, 'b', [1]⟩] 0 'b' == [1] := by rfl
+example : symbol_arrow_list_to_fun [⟨0, 'a', 1⟩, ⟨0, 'b', 1⟩] 0 'b' = [1] := by rfl
 
-example : symbol_step_multiple_list_to_fun [⟨0, 'a', [1]⟩, ⟨0, 'b', [2]⟩] 0 'a' == [1] := by rfl
+example : symbol_arrow_list_to_fun [⟨0, 'a', 1⟩, ⟨0, 'b', 2⟩] 0 'a' = [1] := by rfl
 
-example : symbol_step_multiple_list_to_fun [⟨0, 'a', [1]⟩, ⟨0, 'b', [2]⟩] 0 'b' == [2] := by rfl
+example : symbol_arrow_list_to_fun [⟨0, 'a', 1⟩, ⟨0, 'b', 2⟩] 0 'b' = [2] := by rfl
 
-example : symbol_step_multiple_list_to_fun [⟨0, 'a', [1]⟩, ⟨0, 'a', [2]⟩] 0 'a' == [1, 2] := by rfl
+example : symbol_arrow_list_to_fun [⟨0, 'a', 1⟩, ⟨0, 'a', 2⟩] 0 'a' = [1, 2] := by rfl
 
 
+structure EpsilonNFA
+  (α : Type)
+  (σ : Type) :
+  Type :=
+  (symbol_fun : σ → α → List σ)
+  (epsilon_arrow_list : List (σ × σ))
+  (starting_state_list : List σ)
+  (accepting_state_list : List σ)
+
+
+def EpsilonNFA.epsilon_closure
+  {α : Type}
+  [DecidableEq α]
+  {σ : Type}
+  [DecidableEq σ]
+  (e : EpsilonNFA α σ)
+  (state_list : List σ) :
+  List σ :=
+  dfs e.epsilon_arrow_list state_list
 
 
 /--
@@ -156,51 +84,42 @@ def EpsilonNFA.eval_one
   (state_list : List σ)
   (symbol : α) :
   List σ :=
-  epsilon_closure e.epsilon_step_list (state_list.map (fun (state : σ) => symbol_step_multiple_list_to_fun e.symbol_step_list state symbol)).join
+  e.epsilon_closure (state_list.map (fun (state : σ) => e.symbol_fun state symbol)).join.dedup
 
 
-def EpsilonNFA.eval_from
-  {α : Type}
-  [DecidableEq α]
-  {σ : Type}
-  [DecidableEq σ]
-  (e : EpsilonNFA α σ)
-  (starting_state_list : List σ) :
-  List α → List σ :=
-  List.foldl e.eval_one starting_state_list
-
-
-/--
-  `EpsilonNFA.eval e cs` := Returns the final list of states that the nondeterministic automaton `e` transitions to if it starts at `e.starting_state_list` and consumes the list of symbols `cs`.
--/
 def EpsilonNFA.eval
   {α : Type}
   [DecidableEq α]
   {σ : Type}
   [DecidableEq σ]
-  (e : EpsilonNFA α σ) :
-  List α → List σ :=
-  e.eval_from e.starting_state_list
+  (e : EpsilonNFA α σ)
+  (input : List α) :
+  List σ :=
+  List.foldl e.eval_one (e.epsilon_closure e.starting_state_list) input
 
 
-example : EpsilonNFA.eval ⟨ [], [], [0], [1] ⟩ ['a'] == [] := by rfl
+#eval EpsilonNFA.eval ⟨ symbol_arrow_list_to_fun [], [], [0], [1] ⟩ ([] : List Char)
 
-example : EpsilonNFA.eval ⟨ [⟨0, 'a', [1]⟩], [], [0], [1] ⟩ ['a'] == [1] := by rfl
+#eval EpsilonNFA.eval ⟨ symbol_arrow_list_to_fun [], [], [0], [1] ⟩ ['a']
 
-example : EpsilonNFA.eval ⟨ [⟨0, 'a', [1]⟩], [], [0], [1] ⟩ ['b'] == [] := by rfl
+example : EpsilonNFA.eval ⟨ symbol_arrow_list_to_fun [⟨0, 'a', 1⟩], [], [0], [1] ⟩ ['a'] == [1] := by rfl
 
-example : EpsilonNFA.eval ⟨ [⟨0, 'a', [1]⟩, ⟨0, 'b', [1]⟩], [], [0], [1] ⟩ ['a'] = [1] := by rfl
+example : EpsilonNFA.eval ⟨ symbol_arrow_list_to_fun [⟨0, 'a', 1⟩], [], [0], [1] ⟩ ['b'] == [] := by rfl
 
-example : EpsilonNFA.eval ⟨ [⟨0, 'a', [1]⟩, ⟨0, 'b', [1]⟩], [], [0], [1] ⟩ ['b'] = [1] := by rfl
+example : EpsilonNFA.eval ⟨ symbol_arrow_list_to_fun [⟨0, 'a', 1⟩, ⟨0, 'b', 1⟩], [], [0], [1] ⟩ ['a'] = [1] := by rfl
 
-example : EpsilonNFA.eval ⟨ [⟨0, 'a', [1]⟩, ⟨0, 'b', [2]⟩], [], [0], [1] ⟩ ['a'] = [1] := by rfl
+example : EpsilonNFA.eval ⟨ symbol_arrow_list_to_fun [⟨0, 'a', 1⟩, ⟨0, 'b', 1⟩], [], [0], [1] ⟩ ['b'] = [1] := by rfl
 
-example : EpsilonNFA.eval ⟨ [⟨0, 'a', [1]⟩, ⟨0, 'b', [2]⟩], [], [0], [1] ⟩ ['b'] = [2] := by rfl
+example : EpsilonNFA.eval ⟨ symbol_arrow_list_to_fun [⟨0, 'a', 1⟩, ⟨0, 'b', 2⟩], [], [0], [1] ⟩ ['a'] = [1] := by rfl
 
-example : EpsilonNFA.eval ⟨ [⟨0, 'a', [1]⟩, ⟨0, 'a', [2]⟩], [], [0], [1] ⟩ ['a'] = [2, 1] := by rfl
+example : EpsilonNFA.eval ⟨ symbol_arrow_list_to_fun [⟨0, 'a', 1⟩, ⟨0, 'b', 2⟩], [], [0], [1] ⟩ ['b'] = [2] := by rfl
+
+example : EpsilonNFA.eval ⟨ symbol_arrow_list_to_fun [⟨0, 'a', 1⟩, ⟨0, 'a', 2⟩], [], [0], [1] ⟩ ['a'] = [2, 1] := by rfl
 
 
-#eval EpsilonNFA.eval ⟨ [], [⟨ 0, [1] ⟩ ], [0], [1] ⟩ ['a']
+#eval EpsilonNFA.eval ⟨ symbol_arrow_list_to_fun [], [⟨ 0, 1 ⟩], [0], [1] ⟩ ([] : List Char)
+
+#eval EpsilonNFA.eval ⟨ symbol_arrow_list_to_fun [], [⟨ 0, 1 ⟩], [0], [1] ⟩ ['a']
 
 
 def EpsilonNFA.accepts
